Prova formal do bubble sort concluido

bubblesort.hs
@@ -1,0 +1,70 @@
+module Bubblesort where
+
+import qualified Prelude
+
+__ :: any
+__ = Prelude.error "Logical or arity value used"
+
+and_rect :: (() -> () -> a1) -> a1
+and_rect f =
+  f __ __
+
+and_rec :: (() -> () -> a1) -> a1
+and_rec =
+  and_rect
+
+data Bool =
+   True
+ | False
+
+data Nat =
+   O
+ | S Nat
+
+data List a =
+   Nil
+ | Cons a (List a)
+
+type Sig a = a
+  -- singleton inductive, whose constructor was exist
+  
+sig_rect :: (a1 -> () -> a2) -> a1 -> a2
+sig_rect f s =
+  f s __
+
+sig_rec :: (a1 -> () -> a2) -> a1 -> a2
+sig_rec =
+  sig_rect
+
+leb :: Nat -> Nat -> Bool
+leb n m =
+  case n of {
+   O -> True;
+   S n' -> case m of {
+            O -> False;
+            S m' -> leb n' m'}}
+
+bubble :: (List Nat) -> List Nat
+bubble l =
+  and_rec (\_ _ l0 ->
+    let {
+     hrec l1 =
+       case l1 of {
+        Nil -> Nil;
+        Cons n l2 ->
+         case l2 of {
+          Nil -> Cons n Nil;
+          Cons n0 l3 ->
+           case leb n n0 of {
+            True ->
+             sig_rec (\rec_res _ -> Cons n rec_res) (hrec (Cons n0 l3));
+            False ->
+             sig_rec (\rec_res _ -> Cons n0 rec_res) (hrec (Cons n l3))}}}}
+    in hrec l0) l
+
+bs :: (List Nat) -> List Nat
+bs l =
+  case l of {
+   Nil -> Nil;
+   Cons h l' -> bubble (Cons h (bs l'))}
+
